-

MkDoc/MkDoc.fst
@@ -39,9 +39,183 @@ let rec liststring_of_term (t: term): Tac (list (string * string))
       | _   -> ["doc:liststring_of_term:error1", concat "|" (map (fun (x, _) -> term_to_string x) args)]
     )
     else []
-    
+
+
+let mk (k: string) (args: list (string * jsonValue))
+  = JsonObject (("kind", JsonString k)::args)
+
+let vconst_to_json (cst: vconst): Tac jsonValue
+  = match cst with
+  | C_Unit      -> mk "unit" []
+  | C_Int     i -> mk "int" ["value", JsonNumber (DecimalNumber i 0 0)]
+  | C_True      -> mk "bool" ["value", JsonBool true]
+  | C_False     -> mk "bool" ["value", JsonBool false]
+  | C_String  s -> mk "string" ["value", JsonString s]
+  | C_Range   r -> mk "range" ["value", JsonString "not supported"]
+  | C_Reify     -> mk "reify" []
+  | C_Reflect n -> mk "reflect" ["name", JsonArray (map JsonString n)]
+
+let fv_to_json fv = JsonArray (map JsonString (inspect_fv fv))
+
+let maybe_to_json #a (f: a -> Tac jsonValue) (v: option a): Tac jsonValue
+ = match v with
+ | Some v -> f v
+ | None   -> JsonNull
+
+let rec term_to_json' (deep: nat) (t: term): Tac jsonValue
+  = if deep > 6 then mk "error" ["detail", JsonString "too deep"]
+    else
+  ( match inspect t with
+  | Tv_Var bv     -> bv_to_json deep "var" bv
+  | Tv_BVar bv    -> bv_to_json deep "bvar" bv
+  | Tv_FVar fv    -> mk "fvar" ["value", fv_to_json fv]
+  | Tv_App f x    -> 
+    let f, args = collect_app t in
+    mk "app" [ "function", term_to_json' (deep + 1) f
+             ; "args", JsonArray (
+               T.map (
+                 fun (arg, qual) -> 
+                   JsonObject 
+                     [ "qualifier", aqual_to_json deep qual
+                     ; "term", term_to_json' (deep + 1) arg
+                     ]
+               ) args)
+             ]
+  | Tv_Abs _ _    -> 
+    let bds, body = collect_abs t in
+    mk "abs" [ "body", term_to_json' (deep + 1) t
+             ; "args", JsonArray (
+               T.map (
+                 fun (arg, qual) -> 
+                   JsonObject 
+                     [ "qualifier", aqual_to_json deep qual
+                     ; "bv", bv_to_json deep "binder" arg 
+                     ]
+               ) (map inspect_binder bds))
+             ]
+  | Tv_Arrow _ _  -> 
+    let typs, c = collect_arr t in
+    mk "arrow" [ "comp", comp_to_json c
+               ; "args", JsonArray (T.map (term_to_json' (deep + 1)) typs)
+               ]
+  | Tv_Type ()    -> mk "Type" []
+  | Tv_Refine x t -> mk "refine"
+    [ "var", bv_to_json deep "bv" x
+    ; "refinement", term_to_json' (deep + 1) t
+    ]
+  | Tv_Const cst  -> vconst_to_json cst
+  | Tv_Uvar i t   -> mk "uvar" ["index", JsonNumber (DecimalNumber i 0 0)]
+  | Tv_Let r attrs b t1 t2 -> 
+      mk "let" 
+      [ "recursive", JsonBool r
+      ; "attributes", JsonArray (T.map (term_to_json' (deep + 1)) attrs)
+      ; "name", bv_to_json deep "bv" b
+      ; "definition", term_to_json' (deep + 1) t1
+      ; "type", term_to_json' (deep + 1) t2
+      ]
+  | Tv_Match t branches    -> 
+      mk "match"
+      [ "term", term_to_json' (deep + 1) t
+      ; "branches", JsonArray (T.map
+        (fun (patt, t) -> 
+          JsonObject
+            [ "pattern", pattern_to_json deep patt
+            ; "term", term_to_json' (deep + 1) t
+            ]
+        )
+        branches)
+      ]
+  | Tv_AscribedT e t tt -> mk "ascribed_term"
+                 [ "e", term_to_json' (deep + 1) e
+                 ; "t", (term_to_json' (deep + 1) t)
+                 ; "tt", maybe_to_json (term_to_json' (deep + 1)) tt]
+  | Tv_AscribedC e t tt -> mk "ascribed_comp"
+                 [ "e", (term_to_json' (deep + 1)) e
+                 ; "t", comp_to_json t
+                 ; "tt", maybe_to_json (term_to_json' (deep + 1)) tt]
+  | Tv_Unknown -> mk "unknown" []
+  )
+and bv_to_json deep (n: string) (b: bv): Tac jsonValue =
+  let b = inspect_bv b in
+  mk n
+    ["name", JsonString b.bv_ppname
+    ;"type", (term_to_json' (deep + 1)) b.bv_sort]
+and aqual_to_json deep (q: aqualv): Tac jsonValue =
+  match q with
+  | Q_Explicit -> JsonObject ["kind", JsonString "explicit"]
+  | Q_Implicit -> JsonObject ["kind", JsonString "implicit"]
+  | Q_Meta t   -> JsonObject ["kind", JsonString "meta"; "resolver", term_to_json' (deep + 1) t]
+and comp_to_json (c: comp): Tac jsonValue =
+  match inspect_comp c with
+  | C_Total ret decr -> JsonObject ["kind", JsonString "total"]
+  | C_Lemma pre post -> JsonObject ["kind", JsonString "lemma"]
+  | C_Unknown   -> JsonObject
+    [ "kind", JsonString "unknown"
+    ; "term", JsonString (comp_to_string c)]
+and pattern_to_json deep (c: pattern): Tac jsonValue =
+  match c with
+  | Pat_Constant c -> mk "constant" [ "value", vconst_to_json c]
+  | Pat_Cons fv l -> 
+             mk "constructor"
+             [ "constructor", fv_to_json fv
+             ; "args", JsonArray (T.map (fun (a, _) -> pattern_to_json deep a) l)] 
+  | Pat_Var bv -> mk "var" [ "name", bv_to_json (deep + 1) "bv" bv ]
+  | Pat_Wild bv -> mk "wild" [ "name", bv_to_json (deep + 1) "bv" bv ]
+  | Pat_Dot_Term bv term -> mk "dot" [ "name", bv_to_json (deep + 1) "bv" bv
+                                    ; "term", term_to_json' (deep + 1) term]
+
+let xxx: string =
+  _ by (
+ let fv = (`(
+  forall x. true
+   // h: Prims.squash (forall (x: t). pred x) -> x: t -> int//Prims.Tot (Prims.squash (pred x))
+ )) in
+ let json = term_to_json' 0 fv in
+ // let json = trytac (fun () -> term_to_json_native fv) in
+ // let json = match json with | Some x -> x | None -> JsonNull in  
+ let str  = stringify json "   " in
+ exact (quote str)
+ )
+
+
+
+let rec hasPrefix (#a: eqtype) (l1 l2: list a) =
+  match l1, l2 with
+  | [], _ -> true
+  | (hd1::tl1), (hd2::tl2) -> hd1 = hd2 && hasPrefix tl1 tl2
+  | _ -> false
+
+
+let hasPrefixStr s1 s2 = hasPrefix (list_of_string s1) (list_of_string s2)
+
+
+let term_to_json (excludeNames: list string) name (t: term): Tac jsonValue
+  = let err msg = mk "error" ["detail", JsonString "term_to_json failed, this is probably due to an unknown constant"; "message", JsonString msg] in
+    if
+      (
+        Some? (find (fun bl -> hasPrefixStr bl name) excludeNames)
+      )
+    then (mk "PrimsEffect" ["name", JsonString name])
+    else
+    ( try (
+          term_to_json' 0 t
+          // match trytac (fun () -> term_to_json' 0 t) with
+          // | Some x -> x
+          // | None   -> err "trytac failed"
+      )
+      with | TacticFailure s -> err s
+           | _ -> err "?"
+    )
+
+module SRL = Data.Serialize
+let term_to_json_native_adapt (t: term): Tac SRL.serialized
+   = SRL.serialize (term_to_json [] "***" t)
 [@plugin]
-let getTypes_asJSON (matchingAttr: option term): Tac jsonValue
+let term_to_json_native (t: term): Tac jsonValue
+   = SRL.deserialize (term_to_json_native_adapt t)
+
+[@plugin]
+let getTypes_asJSON (excludeNames: list string) (matchingAttr: option term): Tac jsonValue
   = let names 
         = match matchingAttr with
         | Some m -> lookup_attr m (top_env ())
@@ -72,6 +246,11 @@ let getTypes_asJSON (matchingAttr: option term): Tac jsonValue
             let doc = find (Inl?) attrs in
             let show_def = find (Inr?) attrs in
             JsonObject [
+                 "type_detailed", (
+                             dump (">>>" ^ (concat "." name));
+                             let x = (try (term_to_json excludeNames (concat "." name) typ) with
+                              |_ -> JsonNull) in x
+                             );
                  "type", JsonString (term_to_string typ);
                  "doc", ( match doc with
                         | Some (Inl (desc, args)) -> 
@@ -91,9 +270,9 @@ let getTypes_asJSON (matchingAttr: option term): Tac jsonValue
     ) names)
 
 [@plugin]
-let export_types_to_file (matchingAttr: option term) filepath: Tac unit
-  =  let o = getTypes_asJSON matchingAttr
-  in let json = stringify o "" 
+let export_types_to_file (excludeNames: list string) (matchingAttr: option term) filepath: Tac unit
+  =  let o = getTypes_asJSON excludeNames matchingAttr
+  in let json = stringify o "  " 
   in let _ = launch_process "sh" ["-c"; "cat - > " ^ filepath] json
   in ()
 
