Data/Serialize/Data.Serialize.MakeNative.fst
@@ -1,0 +1,88 @@
+module Data.Serialize.MakeNative
+
+open FStar.Tactics
+module L = FStar.List.Tot
+
+open Data.Serialize.Helpers
+open Data.Serialize.Helpers.Serialized
+open Data.Serialize.Types
+open Data.Serialize.Typeclasses
+open Data.Serialize.Rep
+
+let _UNSAFE_flag_is_compiled_rewriter (): Lemma (false == true) = admit ()
+let _UNSAFE_flag_is_compiled_rewriter_term = `_UNSAFE_flag_is_compiled_rewriter
+// [@(postprocess_for_extraction_with (fun _ -> apply_lemma (`_UNSAFE_flag_is_compiled_rewriter)))]
+// let flag_is_in_compiled_context = false
+
+// [@plugin]
+// let is_this_module_compiled () = flag_is_in_compiled_context
+
+let plugin_term = `plugin
+
+let mk_native_version (f: term) (nativeName: string) (args: list bool) (return: bool) =
+  let fT = f in
+  let f: fv = fvOf f in
+  let flag: name = nameCurMod' (inspect_fv f) (fun _ -> "flag_is_in_compiled_context") in
+  let flagT:term = pack (Tv_FVar (pack_fv flag)) in
+  let is_this_module_compiled: name = nameCurMod' (inspect_fv f) (fun _ -> "is_this_module_compiled") in
+  let is_this_module_compiledT:term = pack (Tv_FVar (pack_fv is_this_module_compiled)) in
+  let flag_generate = match lookup_typ (top_env ()) flag with
+    | Some _ -> []
+    | None   -> (
+      [ set_sigelt_attrs [`(postprocess_for_extraction_with
+                         (fun _ -> apply_lemma _UNSAFE_flag_is_compiled_rewriter_term))]
+        (pack_sigelt (
+          Sg_Let false (pack_fv flag) [] (`bool) (`false)
+        ))
+      ; set_sigelt_attrs [`plugin]
+        (pack_sigelt (
+          Sg_Let false (pack_fv is_this_module_compiled) [] (`(unit -> bool))
+            (mk_abs [fresh_binder (`unit)] flagT)
+        ))]
+    )
+  in
+  let _  = lookup_typ (top_env ()) flag in
+  let all = map (fun t -> fresh_binder (`_), t) args in
+  let binders = L.map fst all in
+  let body = mk_e_app fT (
+    map (fun (b, isS) -> 
+      if isS
+      then call1 (`deserialize) (binder_to_term b)
+      else binder_to_term b
+      ) all
+  ) in
+  let body = if return then call1 (`serialize) body else body in
+  let f': name = nameCurMod' (inspect_fv f) (fun s -> s ^ "_" ^ nativeName ^ "_native_helper") in
+  let body'_if_fstar: term = mk_e_app (pack (Tv_FVar (pack_fv f'))) (
+    map (fun (b, isS) -> 
+      if isS
+      then call1 (`serialize) (binder_to_term b)
+      else binder_to_term b
+      ) all
+  ) in
+  let body'_if_fstar: term = if return then call1 (`deserialize) body'_if_fstar else body'_if_fstar in
+  let body' = 
+    // (pack (mkIfThenElse (call2 (`(fun (x y: bool) -> x || (~y))) flagT is_this_module_compiledT )
+    //     ( mk_e_app fT
+    //       (map binder_to_term binders)
+    //     )
+        body'_if_fstar
+    //   )
+    // )
+  in
+  let f'': name = nameCurMod' (inspect_fv f) (fun s -> nativeName) in
+  let se = 
+    Sg_Let false (pack_fv f') []
+           (`_) (mk_abs binders body)
+  in let se' = 
+    Sg_Let false (pack_fv f'') []
+           (tc (top_env ()) fT)
+           (mk_abs binders body')
+  in let ll = flag_generate @ [
+    set_sigelt_attrs [plugin_term] (pack_sigelt se)
+  ; pack_sigelt se'
+ ] in
+ dump (term_to_string (quote ll));
+ ll
+
+
