MkDoc/Test/MkDoc.Test.fst
@@ -7,6 +7,38 @@ open Data.JSON.Types
 
 open Data.Serialize.Helpers
 
+// let forallInstSq () = pack (Tv_FVar (pack_fv ["FStar"; "Tactic"; "Logic"; "__forall_inst_sq"]))
+
+let t = magic ()
+let pred = magic ()
+
+open FStar.Tactics.PatternMatching
+let a: string = _ by (
+  let x = tc (top_env ()) (`(forall x. true)) in
+  let x = term_head (`(forall x. true)) in
+  exact (quote x)
+)
+
+
+let x: string =
+  _ by (
+ let fv = (`(
+  forall x. true
+   // h: Prims.squash (forall (x: t). pred x) -> x: t -> int//Prims.Tot (Prims.squash (pred x))
+ )) in
+ let json = term_to_json_native fv in
+ // let json = trytac (fun () -> term_to_json_native fv) in
+ // let json = match json with | Some x -> x | None -> JsonNull in  
+ let str  = stringify json "   " in
+ exact (quote str)
+ )
+
+let exclude = ["Prims.Pure"; "Prims.Admit"; "Prims.Ghost"; "Prims.GHOST"
+       ; "Prims.GTot"; "Prims.Lemma"; "Prims.PURE"; "Prims.M"
+       ; "Prims.Tot"; "FStar.ST"; "FStar.Tactics.Effect"; "FStar.Classical"
+       ; "FStar.All" //; "FStar.Pervasives.Div"; "FStar.Pervasives.ALL_h"
+       ; "FStar.Pervasives"]
+
 [@(Doc "s" ["x: adasd", "asd"]) show_def_in_doc]
 type monessai =
   | A : int -> monessai
@@ -15,7 +47,9 @@ type monessai =
 let hey x = x + 1
 
 let _: unit = _ by (
-  export_types_to_file None "result.json";
+  export_types_to_file exclude None "result.json";
   exact (`())
 )
+
+
 
