Data/JSON/default.nix
@@ -1,1 +1,2 @@
 ((import <nixpkgs> {}).fstar-package-manager (import ./fstar-package.nix)).build
+// {doc = "test";}
